Improve how errors are reported from tests
Also changed the structure of tests so the type of the tests is
obviously what we want and only the proof is Ltac magic (which just
makes sure vm_compute is used and gives a more useful error message when
a test fails).

src/goose_lang/interpreter/test_config.v
@@ -3,75 +3,54 @@ From Perennial.goose_lang.interpreter Require Import interpret_types.
 From Perennial.goose_lang.interpreter Require Import interpreter.
 From Perennial.goose_lang.interpreter Require Import disk_interpreter.
 
-From Perennial.goose_lang.examples Require Import goose_unittest.
 From Perennial.goose_lang.ffi Require Import disk.
 
 Definition startstate : state := inhabitant.
-
-(* TODO: move/remove these definitions *)
-Definition testRec : expr :=
-  (rec: BAnon BAnon :=
-     #3 + #3).
-
-Definition testLiteralCast: expr :=
-  λ: <>,
-     let: "x" := #2 in
-     (Var "x") + #2.
-
-Definition testIfStatement: expr :=
-  λ: <>,
-     let: "m" := #2 in
-     (if: (Var "m") > #3
-      then #3
-      else #1).
-
-Definition testMatch: val :=
-  λ: "x",
-  match: (Var "x") with
-    InjL "x1" => #3 + (Var "x1")
-  | InjR "x1" => #4 + (Var "x1")
-  end.
 
 (* testing infrastructure *)
 Definition run (p: expr): Error val :=
   fst <$> runStateT (interpret 100 p) startstate.
 
-Notation check_run p := (ltac:(let x := (eval vm_compute in (run p)) in
-                               lazymatch x with
-                               | Works _ ?v => exact v
-                               | Fail _ ?msg => fail "interpreter failed on" p msg
-                               end)) (only parsing).
-
-Compute check_run (AllocN #1 (zero_val uint32T)).
-Compute check_run (returnTwoWrapper #3).
-Compute check_run (testRec #0).
+Tactic Notation "check_run" constr(p) :=
+  let x := (eval vm_compute in (run p)) in
+  lazymatch x with
+  | Works _ ?v => exact v
+  | Fail _ ?msg => fail "interpreter failed on" p msg
+  end.
+Notation check_run p := (ltac:(check_run p)) (only parsing).
 
 Definition runs_to (p: expr) (v: val) :=
   run p = Works _ v.
-Notation "p ~~> v" := (eq_refl : runs_to p v) (at level 70).
+Notation "p ~~> v" := (runs_to p v) (at level 70).
+Ltac test :=
+  match goal with
+  | [ |- runs_to ?p _ ] =>
+    vm_compute;
+    lazymatch goal with
+    | |- Works _ ?v' = Works _ ?v =>
+      reflexivity || fail 0 p "⇝" v' "but expected" v
+    | |- Fail _ ?msg = _ =>
+      fail "interpreter failed on" p msg
+    | |- ?goal =>
+      fail "vm_compute got stuck" goal
+    end
+  end.
+Notation t := ltac:(test) (only parsing).
 
-Example run_testRec := testRec #0 ~~> #6.
+(* these notations make vm_compute'd values more readable *)
+Notation U64_val z := {| u64_car := {| Naive.unsigned := z; Naive._unsigned_in_range := eq_refl |} |}.
+Notation U32_val z := {| u32_car := {| Naive.unsigned := z; Naive._unsigned_in_range := eq_refl |} |}.
+Notation U8_val z := {| u8_car := {| Naive.unsigned := z; Naive._unsigned_in_range := eq_refl |} |}.
 
-Compute (check_run (testIfStatement #())).
-Compute (check_run (testMatch (InjL #2))).
-Compute (check_run (testMatch (InjR #2))).
-Compute (check_run (testLiteralCast #())).
+Module Examples.
+  Coercion Var' := Var.
+  Definition computeSix : val :=
+    (rec: <> <> :=
+       #3 + #3).
+  Definition add2_u32 : val :=
+    (λ: "x", "x" + #(U32 2)).
 
-(* Functions from examples/goose_unittests *)
-Compute (check_run ConstWithArith).
-Compute (check_run (useMap #())).
-Compute (check_run (useSliceIndexing #())).
-Compute (check_run (ReassignVars #())).
-
-(* fails because #333 is a uint64 *)
-Fail Compute (check_run (EncDec32 #333)).
-
-(* Extraction testing:
-
-Require Coq.extraction.Extraction.
-Extraction Language Haskell.
-Extract Inductive bool => "GHC.Base.Bool" [ "GHC.Base.True" "GHC.Base.False" ].
-
-Extraction "tc1.hs" tc1.
-
-*)
+  Example run1 : computeSix #() ~~> #6 := t.
+  Fail Example run1 : computeSix #() ~~> #5 := t.
+  Fail Example run2 : add2_u32 #333 ~~> #(U32 335) := t.
+End Examples.
